src/Init/Data/Iterators/Lemmas/Consumers/Collect.lean
@@ -11,6 +11,8 @@ public import Init.Data.Iterators.Lemmas.Consumers.Monadic.Collect
 public import Init.Data.Iterators.Consumers.Access
 import all Init.Data.Iterators.Consumers.Access
 import all Init.Data.Iterators.Consumers.Collect
+import all Init.Data.Iterators.Consumers.Total
+import all Init.Data.Iterators.Consumers.Monadic.Total
 
 public section
 
@@ -32,6 +34,23 @@ theorem Iter.toListRev_eq_toListRev_toIterM {α β} [Iterator α Id β] [Finite 
   (rfl)
 
 @[simp]
+theorem Iter.ensureTerminationToArray_eq_toArray {α β} [Iterator α Id β] [Finite α Id] [IteratorCollect α Id Id]
+    [LawfulIteratorCollect α Id Id] {it : Iter (α := α) β} :
+    it.ensureTermination.toArray = it.toArray :=
+  (rfl)
+
+@[simp]
+theorem Iter.ensureTerminationToList_eq_toList {α β} [Iterator α Id β] [Finite α Id] [IteratorCollect α Id Id]
+    [LawfulIteratorCollect α Id Id] {it : Iter (α := α) β} :
+    it.ensureTermination.toList = it.toList :=
+  (rfl)
+
+@[simp]
+theorem Iter.ensureTerminationToListRev_eq_toListRev {α β} [Iterator α Id β] [Finite α Id]
+    {it : Iter (α := α) β} : it.ensureTermination.toListRev = it.toListRev :=
+  (rfl)
+
+@[simp]
 theorem IterM.toList_toIter {α β} [Iterator α Id β] [Finite α Id] [IteratorCollect α Id Id]
     {it : IterM (α := α) Id β} :
     it.toIter.toList = it.toList.run :=
@@ -50,10 +69,22 @@ theorem Iter.toList_toArray {α β} [Iterator α Id β] [Finite α Id] [Iterator
   simp [toArray_eq_toArray_toIterM, toList_eq_toList_toIterM, ← IterM.toList_toArray]
 
 @[simp]
+theorem Iter.toList_ensureTerminationToArray {α β} [Iterator α Id β] [Finite α Id]
+    [IteratorCollect α Id Id] [LawfulIteratorCollect α Id Id] {it : Iter (α := α) β} :
+    it.ensureTermination.toArray.toList = it.toList := by
+  rw [ensureTerminationToArray_eq_toArray, toList_toArray]
+
+@[simp]
 theorem Iter.toArray_toList {α β} [Iterator α Id β] [Finite α Id] [IteratorCollect α Id Id]
     [LawfulIteratorCollect α Id Id] {it : Iter (α := α) β} :
     it.toList.toArray = it.toArray := by
   simp [toArray_eq_toArray_toIterM, toList_eq_toList_toIterM, ← IterM.toArray_toList]
+
+@[simp]
+theorem Iter.toArray_ensureTerminationToList {α β} [Iterator α Id β] [Finite α Id]
+    [IteratorCollect α Id Id] [LawfulIteratorCollect α Id Id] {it : Iter (α := α) β} :
+    it.ensureTermination.toList.toArray = it.toArray := by
+  rw [ensureTerminationToList_eq_toList, toArray_toList]
 
 @[simp]
 theorem Iter.reverse_toListRev [Iterator α Id β] [Finite α Id]
@@ -62,10 +93,21 @@ theorem Iter.reverse_toListRev [Iterator α Id β] [Finite α Id]
     it.toListRev.reverse = it.toList := by
   simp [toListRev_eq_toListRev_toIterM, toList_eq_toList_toIterM, ← IterM.reverse_toListRev]
 
+@[simp]
+theorem Iter.reverse_ensureTerminationToListRev [Iterator α Id β] [Finite α Id]
+    [IteratorCollect α Id Id] [LawfulIteratorCollect α Id Id] {it : Iter (α := α) β} :
+    it.ensureTermination.toListRev.reverse = it.toList := by
+  rw [ensureTerminationToListRev_eq_toListRev, reverse_toListRev]
+
 theorem Iter.toListRev_eq {α β} [Iterator α Id β] [Finite α Id] [IteratorCollect α Id Id]
     [LawfulIteratorCollect α Id Id] {it : Iter (α := α) β} :
     it.toListRev = it.toList.reverse := by
   simp [Iter.toListRev_eq_toListRev_toIterM, Iter.toList_eq_toList_toIterM, IterM.toListRev_eq]
+
+theorem Iter.ensureTerminationToListRev_eq {α β} [Iterator α Id β] [Finite α Id]
+    [IteratorCollect α Id Id] [LawfulIteratorCollect α Id Id] {it : Iter (α := α) β} :
+    it.ensureTermination.toListRev = it.toList.reverse := by
+  rw [ensureTerminationToListRev_eq_toListRev, toListRev_eq]
 
 theorem Iter.toArray_eq_match_step {α β} [Iterator α Id β] [Finite α Id] [IteratorCollect α Id Id]
     [LawfulIteratorCollect α Id Id] {it : Iter (α := α) β} :
@@ -78,6 +120,14 @@ theorem Iter.toArray_eq_match_step {α β} [Iterator α Id β] [Finite α Id] [I
   generalize it.toIterM.step.run = step
   cases step.inflate using PlausibleIterStep.casesOn <;> simp
 
+theorem Iter.ensureTerminationToArray_eq_match_step {α β} [Iterator α Id β] [Finite α Id] [IteratorCollect α Id Id]
+    [LawfulIteratorCollect α Id Id] {it : Iter (α := α) β} :
+    it.ensureTermination.toArray = match it.step.val with
+      | .yield it' out => #[out] ++ it'.toArray
+      | .skip it' => it'.toArray
+      | .done => #[] := by
+  rw [ensureTerminationToArray_eq_toArray, toArray_eq_match_step]
+
 theorem Iter.toList_eq_match_step {α β} [Iterator α Id β] [Finite α Id] [IteratorCollect α Id Id]
     [LawfulIteratorCollect α Id Id] {it : Iter (α := α) β} :
     it.toList = match it.step.val with
@@ -87,6 +137,14 @@ theorem Iter.toList_eq_match_step {α β} [Iterator α Id β] [Finite α Id] [It
   rw [← Iter.toList_toArray, Iter.toArray_eq_match_step]
   split <;> simp [Iter.toList_toArray]
 
+theorem Iter.ensureTerminationToList_eq_match_step {α β} [Iterator α Id β] [Finite α Id] [IteratorCollect α Id Id]
+    [LawfulIteratorCollect α Id Id] {it : Iter (α := α) β} :
+    it.ensureTermination.toList = match it.step.val with
+      | .yield it' out => out :: it'.toList
+      | .skip it' => it'.toList
+      | .done => [] := by
+  rw [ensureTerminationToList_eq_toList, toList_eq_match_step]
+
 theorem Iter.toListRev_eq_match_step {α β} [Iterator α Id β] [Finite α Id] {it : Iter (α := α) β} :
     it.toListRev = match it.step.val with
       | .yield it' out => it'.toListRev ++ [out]
@@ -95,6 +153,13 @@ theorem Iter.toListRev_eq_match_step {α β} [Iterator α Id β] [Finite α Id] 
   rw [Iter.toListRev_eq_toListRev_toIterM, IterM.toListRev_eq_match_step, Iter.step, Id.run_bind]
   generalize it.toIterM.step.run = step
   cases step.inflate using PlausibleIterStep.casesOn <;> simp
+
+theorem Iter.ensureTerminationToListRev_eq_match_step {α β} [Iterator α Id β] [Finite α Id] {it : Iter (α := α) β} :
+    it.ensureTermination.toListRev = match it.step.val with
+      | .yield it' out => it'.toListRev ++ [out]
+      | .skip it' => it'.toListRev
+      | .done => [] := by
+  rw [ensureTerminationToListRev_eq_toListRev, toListRev_eq_match_step]
 
 theorem Iter.getElem?_toList_eq_atIdxSlow? {α β}
     [Iterator α Id β] [Finite α Id] [IteratorCollect α Id Id] [LawfulIteratorCollect α Id Id]
